rejnfrje

LeanGrow/Src/Data/SetTrie/Theory/Model.lean
@@ -2,6 +2,9 @@
 
 import LeanGrow.Src.Data.SetTrie.Operations
 import Mathlib.Data.Finset.Card
+import Mathlib.Data.Finset.Sort -- for repr instance
+import Mathlib.Data.Finset.Union
+import Mathlib.Data.Finset.Insert
 
 open Finset
 
@@ -16,11 +19,24 @@ def SetTrie.fold {γ : Type _} (c : SetTrie α β) (init : γ) (merge : γ → �
   | .node q c => merge (c.foldl (fun s t => (SetTrie.fold t s merge)) init) q
   | .leaf _ => init
 
+#check 1
+
+def SetTrie.mapMerge {γ : Type _} (c : SetTrie α β)
+  (mergeR : List γ → γ) (mergeN : β → List γ → γ) (base : γ) : γ :=
+  match c with
+  | .root c => mergeR <| c.map (SetTrie.mapMerge · mergeR mergeN base)
+  | .node q c => mergeN q <| c.map (SetTrie.mapMerge · mergeR mergeN base)
+  | .leaf _ => base
+
+
 
 namespace StudyST
 
 abbrev fold {γ : Type _} (c : StudyST α) (init : γ) (merge : γ → (Finset α) → γ) : γ :=
   SetTrie.fold c init merge
+
+abbrev mapMerge {γ : Type _} (c : StudyST α) (mergeR : List γ → γ) (mergeN : (Finset α) → List γ → γ) (base : γ) : γ :=
+  SetTrie.mapMerge c mergeR mergeN base
 
 def univ (st : StudyST α) : Finset α :=
   st.fold ∅ (fun x y => x ∪ y)
@@ -41,4 +57,22 @@ def hasNode (st : StudyST α) (n : Finset α) : Prop :=
   st.someNode (fun x => n = x)
 
 def sets (st : StudyST α) : Finset (Finset α) :=
-  st.fold ∅ (fun x y => x.image (fun z => z ∪ y))
+  st.mapMerge
+    (fun c => c.foldl (fun x y => x ∪ y) (∅ : Finset (Finset α)))
+    (fun q c => (c.foldl (fun x y => x ∪ y) ∅).image (fun z => q ∪ z))
+    {∅}
+
+
+#check 1
+
+
+def test : StudyST Nat :=
+  .root
+    [.node {1,2}
+        [.node {3} [.leaf ()],
+         .node {4} [.leaf ()]],
+     .node {5} [.leaf ()]
+    ]
+
+
+#eval test.sets
